Preservation for function
* Preservation for fun : nil case

* add generalize

* Rewrite preservation for Values

* Small fix

* Add weakening

* Add weakening theorem

* Solve all weakening thearems

* some more

* small fix

* Add weakening apply and equality

* fix names

* Avoid sorry and fix naming

LocalLang/TypingGuarantees.lean
@@ -2,17 +2,119 @@ import LocalLang.AST
 import LocalLang.Semantics
 import LocalLang.Types
 import LocalLang.Typing
+import LocalLang.Weakening
 
-def EnvRespectsCtx (Γ : TypeContext) (V : Env) : Prop := sorry
+namespace TypeContext
 
--- TODO: prove
--- TODO: V and Γ should be related
-theorem preservation (Γ : TypeContext) (e e' : Expr) (ty : LLType)
-    (h_env_respects : EnvRespectsCtx Γ V)
-  : Expr.TypeJdg Γ e ty → HeadSmallStep V e e' → Expr.TypeJdg Γ e' ty := sorry
+def respects_env (Γ : TypeContext) (V : Env) : Prop :=
+  ∀ (x : String) (v : Value), V[x]? = v → ∃ ty, Γ[x]? = some ty ∧ v.TypeJdg ty
 
--- Progress: if TypeJdg Γ e ty, then e can take a step.
--- TODO: formalize
+end TypeContext
 
--- TODO: Also interesting:
--- if TypeJdg Γ e ty, then eval e succeeds
+namespace Env
+
+def respects_type_context (V : Env) (Γ : TypeContext) : Prop :=
+  ∀ (x : String) (ty : LLType), Γ[x]? = some ty
+  → ∃ v, V[x]? = some v ∧ v.TypeJdg ty
+
+end Env
+
+theorem addBindings_typing (Γ : TypeContext) {ps : List String} {es : List Expr}
+                           (bd : Expr) (ty : LLType)
+                           (H_len : ps.length = es.length) (arg_types : List LLType)
+  (H_args : Expr.TypeJdgList Γ es arg_types)
+  (body_jdg : Expr.TypeJdg Γ (Expr.value (Value.closure ps bd)) (LLType.func arg_types ty))
+  : Expr.TypeJdg Γ (Expr.addBindings ps es bd H_len) ty := by
+  generalize qs_equality : (ps.zip es) = qs
+  induction qs generalizing ps es bd arg_types with
+  | nil =>
+          rw [Expr.addBindings, qs_equality]
+          rw [List.zip_eq_nil_iff] at qs_equality
+          have h_ps_nil : ps = [] := by
+           cases qs_equality with
+           | inl h => apply h
+           | inr h =>
+             rw [h] at H_len
+             exact List.eq_nil_of_length_eq_zero H_len
+          cases body_jdg with
+          | jdg_value h_value =>
+            cases h_value with
+            | jdg_closure body_jdg' =>
+              rw [h_ps_nil] at body_jdg'
+              apply weakening_expr (empty_subcontext Γ) body_jdg'
+  | cons head tail ih =>
+    cases ps with
+    | nil => simp at qs_equality
+    | cons p ps' =>
+      cases es with
+      | nil => simp at qs_equality
+      | cons e es' =>
+          rw [List.zip_cons_cons, List.cons.injEq] at qs_equality
+          have h_head : (p, e) = head := qs_equality.left
+          have h_tail : ps'.zip es' = tail := qs_equality.right
+          have H_len' : ps'.length = es'.length := by
+                  simpa [List.length] using H_len
+
+          unfold Expr.addBindings
+          simp [List.foldl_cons]
+
+          change Expr.TypeJdg Γ (Expr.addBindings ps' es' (Expr.letIn p e bd) H_len') ty
+          cases H_args with
+          | cons h_e_t h_es' =>
+            rename_i head_arg_type arg_types
+            cases body_jdg with
+            | jdg_value body_jdg' =>
+              cases body_jdg' with
+              | jdg_closure H_body_jdg H_len_all =>
+                apply ih
+                · exact h_es'
+                · apply Expr.TypeJdg.jdg_value
+                  apply Value.TypeJdg.jdg_closure
+                  · have h_zip : (p :: ps').zip (head_arg_type :: arg_types)
+                      = (p, head_arg_type) :: (ps'.zip arg_types) := rfl
+                    rw [h_zip] at H_body_jdg
+                    apply Expr.TypeJdg.jdg_let_in (ty₁ := head_arg_type)
+                    · apply weakening_expr _ h_e_t
+                      sorry
+                    · sorry
+                  · simp [List.length] at H_len_all
+                    exact H_len_all
+                · exact h_tail
+
+theorem preservation (env : Env) (Γ : TypeContext) (e e' : Expr) (ty : LLType)
+    (h_env_respects : Γ.respects_env env)
+  : Expr.TypeJdg Γ e ty → HeadSmallStep env e e' → Expr.TypeJdg Γ e' ty := by
+    intro h_jdg b
+    induction b
+    · -- const_step
+      cases h_jdg
+      apply Expr.TypeJdg.jdg_value
+      apply Value.TypeJdg.jdg_nat
+    · -- var_step
+      rename_i env n a relΓ
+      cases h_jdg
+      unfold TypeContext.respects_env at h_env_respects
+      let ent_ctx_link := h_env_respects n a relΓ
+      constructor
+      rename_i relΓJd
+      rcases ent_ctx_link with ⟨ty', H_ty'_in_ctx, H_a_type_jdg⟩
+      rw [relΓJd] at H_ty'_in_ctx
+      rw [Option.some.inj H_ty'_in_ctx]
+      apply H_a_type_jdg
+    · -- case bin_op_step
+      cases h_jdg
+      rename_i H₁ H₂
+      cases H₂
+      apply Expr.TypeJdg.jdg_value
+      apply Value.TypeJdg.jdg_nat
+    · -- case let_in_const_step
+      cases h_jdg
+      apply Expr.TypeJdg.jdg_value
+      rename_i H₁ H₂
+      cases H₂
+      assumption
+    · -- case fun_step.jdg_fun
+      cases h_jdg
+      rename_i r env es ps bd H_len r_eq arg_types H_args f_jdg
+      rw [r_eq]
+      apply addBindings_typing Γ bd ty H_len arg_types H_args f_jdg
